PolyFun.lean
@@ -113,7 +113,7 @@ import PolyFun.PFunctor.Dynamical.Behavior
 import PolyFun.PFunctor.Dynamical.Bisimulation
 import PolyFun.PFunctor.Dynamical.Combinators
 import PolyFun.PFunctor.Dynamical.Game
-import PolyFun.PFunctor.Dynamical.PointedMachine
+import PolyFun.PFunctor.Dynamical.IOMachine
 import PolyFun.PFunctor.Dynamical.Refinement
 import PolyFun.PFunctor.Dynamical.Responder
 import PolyFun.PFunctor.Dynamical.Run
